chars

NFA.v
@@ -1,72 +1,206 @@
 
-Require Export Str Reg.
+Require Export Lang Reg.
+Unset Strict Implicit.
+Unset Printing Implicit Defensive.
+
+Section NFA.
+Context (L : Lang) (state : finType).
+
+
+hogehoge
 
 
 
+Inductive chars : Type :=
+    | char0  
+    | char1 of char.
 
 
-Record chars {finStr : str}: Type := mkChar {
-    c :> finStr;
-    _ : c ∈ ([set [::x]| x in [set : char]] ∪ [set ϵ]);
-}.
+Notation ϵ_ := char0.  
 
+Definition chars2finStr (c : chars) : finStr :=
+    match c with
+    | char0 => ϵ
+    | char1 a => [:: a]
+    end.
 
+Coercion chars2finStr : chars >-> Finite.sort.
 
-Definition ϵ_ {finStr : str}: chars.
-    apply (mkChar _ ϵ).
-    rewrite inE; apply /orP; right.
-    rewrite inE => //.
-Qed.
+Definition chars_eqb (a b : chars) := 
+    match a, b with
+    | char0 , char0 => true
+    | char1 a_, char1 b_ => a_ == b_
+    | _,_ => false
+    end.
 
-Definition charOf {finStr : str} (a : char) : chars.
+Definition chars_eqAxiom : Equality.axiom chars_eqb.
 Proof.
-    apply (mkChar _ [:: a]).
-    rewrite inE; apply /orP; left.
-    apply /imsetP; exists a => //.
+    move => x y; destruct x,y => /=; try constructor => //.
+    remember (s == s0).
+    destruct b; symmetry in Heqb; constructor.
+    +   move /eqP : Heqb -> => //.
+    +   move => F; inversion F; subst s0.
+        rewrite (eq_refl s) in Heqb; inversion Heqb.
 Qed.
 
-Class nfa {finStr : str} : Type := mkNFA {
-    state : finType;
+Definition chars_eqMixin := EqMixin chars_eqAxiom.
+Canonical chars_eqType := EqType chars chars_eqMixin.
+
+
+
+
+  
+
+
+
+Class nfa := mkNfa{
     Q : {set state};
-    F : {set state};
     p0 : state;
-    δ : state -> chars -> {set state}
+    δ : state -> chars -> {set state};
+    F : {set state};
+    _ : F ⊂ Q;
+    _ : p0 ∈ Q;
 }.
-
-
 
 
 Reserved Notation "p -ϵ-> q"(at level 50).
-Inductive Closure {finStr : str} {N : nfa}: state -> state -> Prop :=
+Inductive Closure {N : nfa}: state -> state -> Prop :=
     | CL_refl p : p -ϵ-> p
     | CL_single p q : q ∈ δ p ϵ_ -> p -ϵ-> q
     | CL_trans p q r : p -ϵ-> q -> q -ϵ-> r ->  p -ϵ-> r
     where "p -ϵ-> q" := (Closure p q).
 
-Axiom closure : forall {finStr : str} {N : nfa}, {set state} -> {set state}.
-Axiom closureP : forall {finStr : str} {N : nfa} (P : {set state}) q,
-    reflect (forall p, p ∈ P -> p -ϵ-> q) (q ∈ closure P).
 
 
-Fixpoint δ' {finStr : str} {N : nfa} (p : state) (s : finStr) : {set state} :=
+Axiom closure : forall {N : nfa}, {set state} -> {set state}.
+Axiom closureP : forall (N : nfa) (P : {set state}) q,
+    reflect (exists p, p ∈ P /\ p -ϵ-> q) (q ∈ closure P).
+
+
+Fixpoint δ' {N : nfa}  (p : state) (s : finStr) : {set state} :=
     match s with
     | [::] => closure [set p]
-    | a :: w => closure (bigcup [set δ x (charOf a) | x in δ' p w])
+    | a :: w => closure (bigcup [set δ x (char1 a) | x in δ' p w])   
     end.
+        
 
-Definition L {finStr : str} (N : nfa) := [set w : finStr | (δ' p0 w ∩ F) == ∅].
+Definition LangOf (N : nfa) := 
+    [set w : finStr | ~~ ((δ' p0 w ∩ F) == ∅)].
 
 
 
+Variable p q : state.
+Definition dQ := [set p; q].
+Definition dF := [set q].
+Hypotheses npq : p <> q.
 
-Section Properties.
+Lemma dFQ : dF ⊂ dQ.
+Proof.
+    apply /subsetP => x /set1P H; subst; apply /set2P; right => //.
+Qed. 
 
-Context (finStr : str) (lo : lang_op finStr)(Σ : lang).
+Lemma pQ : p ∈ dQ.
+Proof.
+    apply /set2P; left => //.
+Qed.
+
+
 
 Theorem reg_nfa :
-    forall l : Σ, Reg l -> exists N : nfa, L N = l.
+    forall l , Reg l -> exists N : nfa, LangOf N = l.
 Proof.
-Admitted.
+    move => l Hl; induction Hl.
+    +   pose N := (mkNfa dQ p (fun _ _ => ∅) ∅ (sub0set dQ) pQ).
+        exists N.
+        rewrite /LangOf.
+        apply extension; apply /subsetP => x. 
+        -   rewrite in_set setI0 => /=.
+            move /eqP => F.
+            contradiction F => //.
+        -   move : (in_set0 x) -> => //.
+    +   pose f := fun (s : state) (c : chars)=> if (c == ϵ_) && (s == p) then [set q] else ∅.
+        pose N := (mkNfa dQ p f dF dFQ pQ).
+        exists N.
+        rewrite /LangOf.
+        apply extension; apply /subsetP => w.        
+        -   rewrite in_set => /=.
+            move /set0Pn => [x /setIP [Hx /set1P H1]]; subst x.
+            move : q Hx; induction w => q0 Hx.
+            *   apply /set1P => //. 
+            *   move /(closureP N _ q0) : Hx => [p0 [Hp pq0]].
+                move /bigcupP : Hp => /= [Y [pY HY]].
+                move /imsetP : HY => [x Hx Yf]; subst Y.
+                rewrite /f in pY.
+                simpl in pY.
+                rewrite (in_set0 p0) in pY; inversion pY.
+         -  move /set1P ->.
+            rewrite in_set.
+            apply /eqP => /= F.
+            have : (q ∈ ∅).
+                rewrite -F.
+                apply /setIP; split.
+                *   apply /closureP.
+                    exists p; split.
+                    apply /set1P => //.
+                    apply CL_single => /=.
+                    rewrite /f => /=.
+                    rewrite eq_refl.
+                    apply /set1P => //.
+                *   apply /set1P => //.
+            rewrite (in_set0 q) => //.            
+    +   pose f := fun (s : state) (c : chars)=> if (c == char1 a ) && (s == p) then [set q] else ∅.
+        pose N := (mkNfa dQ p f dF dFQ pQ).
+        exists N.
+        rewrite /LangOf.
+        apply extension; apply /subsetP => w; first last.
+        -   move /set1P ->.
+            rewrite in_set => /=.
+            apply /eqP => F.
+            have : (q ∈ ∅).
+                rewrite -F.
+                apply /setIP; split; first last.
+                *   apply /set1P => //.
+                *   apply /closureP.
+                    exists q; split.
+                    +   apply /bigcupP.
+                        exists [set q]; split.
+                        -   apply /set1P => //.
+                        -   apply /imsetP.
+                            exists p.
+                            *   apply /closureP.
+                                exists p; split.
+                                +   apply /set1P => //.
+                                +   constructor.
+                            *   rewrite /f.
+                                rewrite !eq_refl => /=.
+                                by [].
+                    +   constructor.
+            rewrite (in_set0 q) => //.
+        -   rewrite in_set => /=; rewrite /dF.
+            Search setI set0.
+            move /set0Pn => [p0 /setIP [Hp /set1P pF]]; subst p0.
+            induction w.
+            *   move /closureP : Hp => [p1 [/set1P H1 pq]]; subst p1; simpl in pq.
+
+                +   case  (npq H0).
+                +   rewrite /δ /N /f /= in H.
+                    rewrite (in_set0 q) in H; inversion H.
+                +   subst.
+                admit.
+            *   admit. *)
+    +   move : IHHl1 => [NX HX].
+        move : IHHl2 => [NY HY].
+        inversion NX as [Qx px fx Fx Hx].
+        inversion NY as [Qy py fy Fy Hy].
+        pose f := fun s c => fx s c ∪ fy s c.
+        pose N := mkNfa state (Qx ∪ Qy) px f (Fx ∪ Fy) (setUSS Hx Hy).
+        exists N.
+        rewrite /LangOf.
+        apply extension; apply /subsetP => z.
+        -   rewrite in_set.
+            move /set0Pn => [xy /setIP [Hxy /setUP bF]].
+            induction z.
+            *   move /closureP : Hxy => [p_ [/set1P pp Hp]]; subst p_; simpl in Hp.
 
 
 
